byteback-core/src/integration/resources/regression/java8/boogie/byteback.dummy.condition.Array.bpl
@@ -1,13 +1,136 @@
+// -------------------------------------------------------------------
+// Heap model
+// -------------------------------------------------------------------
+type Reference;
+
+const ~null: Reference;
+
+type Field a;
+type Store = [Reference]<a>[Field a]a;
+
+var ~heap: Store;
+
+function ~read<a>(h: Store, r: Reference, f: Field a) returns (a)
+{ h[r][f] }
+
+function ~update<a>(h: Store, r: Reference, f: Field a, v: a) returns (Store)
+{ h[r := h[r][f := v]] }
+
+procedure ~new() returns (~ret: Reference);
+
+// -------------------------------------------------------------------
+// Array model
+// -------------------------------------------------------------------
+type Array a = Field [int]a;
+
+const unique ~Array.bool: Array bool;
+
+const unique ~Array.int: Array int;
+
+const unique ~Array.real: Array real;
+
+const unique ~Array.Reference: Array Reference;
+
+const unique ~Array.length: Field int;
+
+function ~lengthof(h: Store, r: Reference) returns (int)
+{
+  ~read(h, r, ~Array.length)
+}
+
+function ~get<a>(h: Store, r: Reference, f: Array a, i: int) returns (a)
+{
+  ~read(h, r, f)[i]
+}
+
+function ~insert<a>(h: Store, r: Reference, f: Array a, i: int, e: a) returns (Store)
+{
+  ~update(h, r, f, ~read(h, r, f)[i := e])
+}
+
+procedure ~array(l: int) returns (~ret: Reference);
+  modifies ~heap;
+  ensures ~read(~heap, ~ret, ~Array.length) == l;
+
+// -------------------------------------------------------------------
+// Binary operators
+// -------------------------------------------------------------------
+function ~cmp<t>(a: t, b: t) returns (int);
+
+axiom (forall i: real, j: real :: i < j <==> ~cmp(i, j) == -1);
+axiom (forall i: real, j: real :: i > j <==> ~cmp(i, j) == 1);
+axiom (forall i: real, j: real :: i == j <==> ~cmp(i, j) == 0);
+
+axiom (forall i: int, j: int :: i < j <==> ~cmp(i, j) == -1);
+axiom (forall i: int, j: int :: i > j <==> ~cmp(i, j) == 1);
+axiom (forall i: int, j: int :: i == j <==> ~cmp(i, j) == 0);
+
+// -------------------------------------------------------------------
+// Prelude definitions
+// -------------------------------------------------------------------
+function ~and(~heap: Store, a: bool, b: bool) returns (bool)
+{ a && b }
+
+function ~or(~heap: Store, a: bool, b: bool) returns (bool)
+{ a || b }
+
+function ~implies(~heap: Store, a: bool, b: bool) returns (bool)
+{ a ==> b }
+
+function ~iff(~heap: Store, a: bool, b: bool) returns (bool)
+{ a <==> b }
+
+function ~lt<t>(~heap: Store, a: t, b:  t) returns (bool);
+axiom (forall ~heap: Store, a: real, b: real :: ~lt(~heap, a, b) <==> a < b);
+axiom (forall ~heap: Store, a: int, b: int :: ~lt(~heap, a, b) <==> a < b);
+
+function ~lte<t>(~heap: Store, a: t, b: t) returns (bool);
+axiom (forall ~heap: Store, a: real, b: real :: ~lte(~heap, a, b) <==> a <= b);
+axiom (forall ~heap: Store, a: int, b: int :: ~lte(~heap, a, b) <==> a <= b);
+
+function ~gt<t>(~heap: Store, a: t, b: t) returns (bool);
+axiom (forall ~heap: Store, a: real, b: real :: ~gt(~heap, a, b) <==> a > b);
+axiom (forall ~heap: Store, a: int, b: int :: ~gt(~heap, a, b) <==> a > b);
+
+function ~gte<t>(~heap: Store, a: t, b: t) returns (bool);
+axiom (forall ~heap: Store, a: real, b: real :: ~gte(~heap, a, b) <==> a >= b);
+axiom (forall ~heap: Store, a: int, b: int :: ~gte(~heap, a, b) <==> a >= b);
+
+function ~eq<t>(~heap: Store, a: t, b: t) returns (bool)
+{ a == b }
+
+// -------------------------------------------------------------------
+// Casting operators
+// -------------------------------------------------------------------
+
+// Casting between primitive types
+function ~int<a>(a) returns (int);
+
+// bool -> int
+axiom ~int(false) == 0;
+axiom ~int(true) == 1;
+
+// real -> int
+// TODO
+
+function ~real<a>(a) returns (real);
+
+// int -> real
+// TODO
+
 procedure byteback.dummy.condition.Array.sum#int$#(as: Reference) returns (~ret: int)
   ensures ~implies(~heap,
-    (forall index: int :: ~and(~heap, ~lt(~heap, index, ~lengthof(~heap, as)), ~gte(~heap, index, 0))),
+    (forall index : int :: ~implies(~heap,
+                        ~and(~heap,
+                         ~lt(~heap, index, ~lengthof(~heap, as)),
+                         ~gte(~heap, index, 0)),
+                        ~gte(~heap, ~get(~heap, as, ~Array.int, index), 0))),
     ~gte(~heap, ~ret, 0));
 {
   var c: int;
   var l4: int;
   c := 0;
   l4 := 0;
-
 label2:
 
   if (l4 >= ~lengthof(~heap, as)) {
